theories/microgv/langtools.v
@@ -1,3 +1,7 @@
 From iris.proofmode Require Export base tactics classes.
 From diris.cgraphs Require Export util.
-Require Export Coq.Logic.Classical.
+From Coq.Logic Require Export FunctionalExtensionality Classical.
+From diris Require Export seplogic.
+From stdpp Require Export gmap.
+
+Ltac inv H := inversion H; clear H; simplify_eq.
