theories/microgv/rtypesystem.v
@@ -1,0 +1,296 @@
+From diris.microgv Require Export langdef.
+
+Inductive vertex := Thread (_:nat) | Barrier (_:nat).
+Definition label : Type := type * type.
+
+(* ----------- *)
+(* Boilerplate *)
+
+(* Canonical Structure vertexO := leibnizO vertex. *)
+Definition labelO := leibnizO label.
+
+Instance vertex_eqdecision : EqDecision vertex.
+Proof.
+  intros [n|n] [m|m]; unfold Decision; destruct (decide (n = m));
+  subst; eauto; right; intro; simplify_eq.
+Qed.
+Instance vertex_countable : Countable vertex.
+Proof.
+  refine (inj_countable' (λ l, match l with
+  | Thread n => inl n
+  | Barrier n => inr n
+  end) (λ l, match l with
+  | inl n => Thread n
+  | inr n => Barrier n
+  end) _); by intros [].
+Qed.
+
+(* End boilerplate *)
+(* --------------- *)
+
+Notation rProp := (hProp vertex labelO).
+
+Definition linbox l (P : rProp) : rProp :=
+  match l with
+  | Lin => P
+  | Unr => □ P
+  end.
+
+Fixpoint rtyped (Γ : env) e t : rProp :=
+  match e with
+  | Val v => vtyped v t
+  | Var x => ∃ Γ', ⌜⌜ env_insert Γ x t Γ' ∧ env_unr Γ' ⌝⌝
+  | Fun x e =>
+      ∃ l t1 t2, ⌜⌜ t = FunT l t1 t2 ⌝⌝  ∗
+      ∃ Γ', ⌜⌜ env_insert Γ' x t1 Γ ∧ (l = Unr -> env_unr Γ) ⌝⌝ ∗
+      linbox l (rtyped Γ' e t2)
+  | App e1 e2 =>
+      ∃ Γ1 Γ2, ⌜⌜ env_split Γ Γ1 Γ2 ⌝⌝ ∗
+      ∃ t1 l,
+      rtyped Γ1 e1 (FunT l t1 t) ∗
+      rtyped Γ2 e2 t1
+  | Unit => ⌜⌜ t = UnitT ∧ env_unr Γ ⌝⌝
+  | Pair e1 e2 =>
+      ∃ Γ1 Γ2, ⌜⌜ env_split Γ Γ1 Γ2 ⌝⌝ ∗
+      ∃ t1 t2, ⌜⌜ t = PairT t1 t2 ⌝⌝ ∗
+      rtyped Γ1 e1 t1 ∗ rtyped Γ2 e2 t2
+  | LetPair e1 e2 =>
+      ∃ Γ1 Γ2, ⌜⌜ env_split Γ Γ1 Γ2 ⌝⌝ ∗
+      ∃ t1 t2,
+      rtyped Γ1 e1 (PairT t1 t2) ∗
+      rtyped Γ2 e2 (FunT Lin t1 (FunT Lin t2 t))
+  | Sum i e =>
+      ∃ n (ts : fin n -> type) (i' : fin n), ⌜⌜ t = SumT n ts ⌝⌝ ∗ ⌜⌜ i = i' ⌝⌝ ∗
+      rtyped Γ e (ts i')
+  | MatchSum n e es =>
+      ∃ Γ1 Γ2, ⌜⌜ env_split Γ Γ1 Γ2 ∧ (n = 0 -> env_unr Γ2)⌝⌝ ∗
+      ∃ ts,
+      rtyped Γ1 e (SumT n ts) ∗
+      (∀ i, rtyped Γ2 (es i) (FunT Lin (ts i) t))
+  | Fork e =>
+      ∃ t1 t2, ⌜⌜ t = FunT Lin t1 t2 ⌝⌝ ∗
+      rtyped Γ e (FunT Lin (FunT Lin t2 t1) UnitT)
+  end
+with vtyped v t :=
+  match v with
+  | FunV x e =>
+      ∃ l t1 t2, ⌜⌜ t = FunT l t1 t2 ⌝⌝ ∗ linbox l (rtyped {[ x := t1 ]} e t2)
+  | UnitV => ⌜⌜ t = UnitT ⌝⌝
+  | PairV v1 v2 =>
+      ∃ t1 t2, ⌜⌜ t = PairT t1 t2 ⌝⌝ ∗
+      vtyped v1 t1 ∗ vtyped v2 t2
+  | SumV i v =>
+      ∃ n ts (i' : fin n), ⌜⌜ t = SumT n ts ∧ i = i' ⌝⌝ ∗
+      vtyped v (ts i')
+  | BarrierV k =>
+      ∃ t1 t2, ⌜⌜ t = FunT Lin t1 t2 ⌝⌝ ∗
+      own_out (Barrier k) ((t1,t2) : labelO)
+  end.
+
+Lemma typed_rtyped Γ e t :
+  ⌜⌜ typed Γ e t ⌝⌝ -∗ rtyped Γ e t.
+Proof.
+  iIntros (H).
+  iInduction e as [] "IH" forall (t Γ H);
+  inv H; simpl; eauto; repeat (iExists _ || iSplitL ""); eauto;
+  try (destruct l; iModIntro); repeat iIntros (?);
+  try iApply ("IH" with "[%]") || iApply ("IH1" with "[%]"); eauto.
+Qed.
+
+(* From stdpp's naive_solver *)
+Ltac simp :=
+  repeat match goal with
+  (**i solve the goal *)
+  | |- _ => fast_done
+  (**i intros *)
+  | |- ∀ _, _ => intro
+  (**i simplification of assumptions *)
+  | H : False |- _ => destruct H
+  | H : _ ∧ _ |- _ =>
+     (* Work around bug https://coq.inria.fr/bugs/show_bug.cgi?id=2901 *)
+     let H1 := fresh in let H2 := fresh in
+     destruct H as [H1 H2]; try clear H
+  | H : ∃ _, _  |- _ =>
+     let x := fresh in let Hx := fresh in
+     destruct H as [x Hx]; try clear H
+  | H : ?P → ?Q, H2 : ?P |- _ => specialize (H H2)
+  | H : Is_true (bool_decide _) |- _ => apply (bool_decide_unpack _) in H
+  | H : Is_true (_ && _) |- _ => apply andb_True in H; destruct H
+  (**i simplify and solve equalities *)
+  | |- _ => progress simplify_eq/=
+  (**i operations that generate more subgoals *)
+  (* | |- _ ∧ _ => split *)
+  (* | |- Is_true (bool_decide _) => apply (bool_decide_pack _) *)
+  (* | |- Is_true (_ && _) => apply andb_True; split *)
+  (* | H : _ ∨ _ |- _ => *)
+     (* let H1 := fresh in destruct H as [H1|H1]; try clear H *)
+  (* | H : Is_true (_ || _) |- _ => *)
+     (* apply orb_True in H; let H1 := fresh in destruct H as [H1|H1]; try clear H *)
+  (**i solve the goal using the user supplied tactic *)
+  end.
+
+Ltac iDestr H := repeat iDestruct H as (?) H; try iDestruct H as %?.
+
+Lemma unrestricted_box v t :
+  unr t -> vtyped v t -∗ □ vtyped v t.
+Proof.
+  iIntros (H) "H".
+  iInduction v as [] "IH" forall (t H); simpl;
+  iDestr "H"; simp; inv H; simp; eauto.
+  - iDestruct "H" as "#H". iModIntro. eauto.
+  - iDestruct "H" as "[H1 H2]".
+    iDestruct ("IH" with "[%] H1") as "H1"; first done.
+    iDestruct ("IH1" with "[%] H2") as "H2"; first done.
+    iDestruct "H1" as "#H1".
+    iDestruct "H2" as "#H2".
+    iModIntro. repeat (iExists _ || iSplitL); eauto.
+  - iDestruct ("IH" with "[%] H") as "H"; first done.
+    iDestruct "H" as "#H". iModIntro. eauto.
+Qed.
+
+Lemma substitution Γ x v tV e t :
+  Γ !! x = Some tV ->
+  vtyped v tV ∗ rtyped Γ e t -∗
+  rtyped (delete x Γ) (subst x v e) t.
+Proof.
+Admitted.
+
+Fixpoint rtyped0 e t : rProp :=
+  match e with
+  | Val v => vtyped v t
+  | Var x => False
+  | Fun x e =>
+      ∃ l t1 t2, ⌜⌜ t = FunT l t1 t2 ⌝⌝ ∗
+      ∃ Γ, ⌜⌜ env_insert Γ x t1 ∅ ⌝⌝ ∗
+      linbox l (rtyped Γ e t2)
+  | App e1 e2 =>
+      ∃ t1 l,
+      rtyped0 e1 (FunT l t1 t) ∗
+      rtyped0 e2 t1
+  | Unit => ⌜⌜ t = UnitT ⌝⌝
+  | Pair e1 e2 =>
+      ∃ t1 t2, ⌜⌜ t = PairT t1 t2 ⌝⌝ ∗
+      rtyped0 e1 t1 ∗ rtyped0 e2 t2
+  | LetPair e1 e2 =>
+      ∃ t1 t2,
+      rtyped0 e1 (PairT t1 t2) ∗
+      rtyped0 e2 (FunT Lin t1 (FunT Lin t2 t))
+  | Sum i e =>
+      ∃ n (ts : fin n -> type) (i' : fin n), ⌜⌜ t = SumT n ts ⌝⌝ ∗ ⌜⌜ i = i' ⌝⌝ ∗
+      rtyped0 e (ts i')
+  | MatchSum n e es =>
+      ∃ ts,
+      rtyped0 e (SumT n ts) ∗
+      (∀ i, rtyped0 (es i) (FunT Lin (ts i) t))
+  | Fork e =>
+      ∃ t1 t2, ⌜⌜ t = FunT Lin t1 t2 ⌝⌝ ∗
+      rtyped0 e (FunT Lin (FunT Lin t2 t1) UnitT)
+  end.
+
+Lemma env_split_empty Γ1 Γ2 :
+  env_split ∅ Γ1 Γ2 <-> Γ1 = ∅ ∧ Γ2 = ∅.
+Proof.
+Admitted.
+
+Lemma env_unr_empty :
+  env_unr ∅.
+Proof.
+Admitted.
+
+Lemma env_insert_empty x t Γ :
+  env_insert ∅ x t Γ <-> False.
+Proof.
+Admitted.
+
+Lemma env_insert_empty' Γ x t1 :
+  env_insert Γ x t1 ∅ <-> Γ = {[ x := t1]}.
+Proof.
+Admitted.
+
+Lemma rtyped_rtyped0 e t :
+  rtyped ∅ e t ⊣⊢ rtyped0 e t.
+Proof.
+  revert t. induction e; intros; simpl;
+  iSplit; iIntros "H";
+  try setoid_rewrite env_split_empty;
+  try setoid_rewrite env_insert_empty; iDestr "H"; simp;
+  try iDestruct "H" as "[H Q]";
+  repeat (iExists _ || iSplit); eauto using env_unr_empty;
+  rewrite ?H ?IHe ?IHe1 ?IHe2; iFrame;
+  iIntros (?); setoid_rewrite H; eauto.
+Qed.
+
+Lemma substitution0 v t1 t2 x e :
+  vtyped v t1 ∗
+  rtyped {[ x := t1 ]} e t2 -∗
+  rtyped0 (subst x v e) t2.
+Proof.
+  rewrite -rtyped_rtyped0.
+  iIntros "[H Q]".
+  assert (∅ = (delete x {[ x := t1 ]} : env)) as ->.
+  { rewrite delete_singleton //. }
+  iApply substitution; last iFrame.
+  rewrite lookup_singleton //.
+Qed.
+
+Lemma pure_preservation e e' t :
+  pure_step e e' ->
+  rtyped0 e t -∗ rtyped0 e' t.
+Proof.
+  intros []; simpl;
+  iIntros "H";
+  try setoid_rewrite env_insert_empty';
+  repeat (iDestr "H" || iDestruct "H" as "[H ?]"); simp;
+  repeat (iExists _ || iSplit); eauto with iFrame.
+  iApply substitution0. iFrame.
+  by destruct l0.
+Qed.
+
+Lemma replacement1 k e B :
+  ctx1 k ->
+  rtyped0 (k e) B -∗ ∃ t, rtyped0 e t ∗ ∀ e', rtyped0 e' t -∗ rtyped0 (k e') B.
+Proof.
+  destruct 1; simpl; iIntros "H";
+  iDestr "H"; try iDestruct "H" as "[H Q]";
+  eauto 8 with iFrame.
+Qed.
+
+Lemma replacement k e B :
+  ctx k ->
+  rtyped0 (k e) B ⊣⊢ ∃ t, rtyped0 e t ∗ ∀ e', rtyped0 e' t -∗ rtyped0 (k e') B.
+Proof.
+  intros Hk.
+  iSplit; iIntros "H"; last first.
+  { iDestruct "H" as (t) "[H Q]". by iApply "Q". }
+  iInduction Hk as [] "IH" forall (B e); simpl.
+  { iExists _. iFrame. eauto. } subst.
+  iDestruct (replacement1 with "H") as (?) "[H R]"; eauto.
+  iDestruct ("IH" with "H") as (?) "[Q H]".
+  iExists _. iFrame. iIntros (?) "?".
+  iApply "R". iApply "H". done.
+Qed.
+
+
+Ltac solve_ctx := solve [iPureIntro; do 2 eexists; split; last done; eauto using ctx, ctx1].
+Ltac solve_step := solve [iPureIntro; do 2 eexists; split; eauto using Ctx_id; simp; eauto using pure_step].
+
+Ltac solve_pr := simp; try (solve_ctx || solve_step).
+
+Lemma pure_progress e t :
+  rtyped0 e t -∗ ⌜ (∃ v, e = Val v) ∨
+    ∃ k e0, (ctx k ∧ e = k e0) ∧
+      ((∃ e', pure_step e0 e') ∨
+       (∃ v, e0 = Fork (Val v)) ∨
+       (∃ v k, e0 = App (Val $ BarrierV k) (Val v))) ⌝.
+Proof.
+  iIntros "H".
+  iInduction e as [] "IH" forall (t); simpl; eauto;
+  iDestr "H";
+  try iDestruct "H" as "[H Q]"; simp;
+  try iDestruct ("IH" with "H") as %H;
+  try iDestruct ("IH1" with "H") as %H;
+  try iDestruct ("IH1" with "Q") as %Q; iRight;
+  try destruct H; solve_pr;
+  try destruct Q; solve_pr;
+  destruct H0; simpl; iDestr "H"; solve_pr.
+Qed.
